\documentclass[letterpaper]{article}

% --- Packages
\usepackage[utf8]{inputenc}
\usepackage[T1]{fontenc}
\usepackage[margin=0.25cm]{geometry}
\usepackage{enumitem}
\usepackage{pdfpages}
\usepackage{multicol}
\usepackage{amsmath}
\usepackage{amssymb}
\usepackage[skip=1pt plus1pt, indent=0pt]{parskip}
\usepackage{enumitem}
\usepackage{graphicx}

% --- Data
\title{Fourier analysis}
\author{Enrique Calderon}
\date{November 2023}

% --- Graphics path
\graphicspath{ {./img/} }

% --- Custom commands
\makeatletter
\let\thetitle\@title
\let\theauthor\@author
\makeatother
\newcommand{\compconj}[1]{%
	\overline{#1}%
}
\newcommand{\divline}{\noindent\makebox[\linewidth]{\rule{\textwidth}{0.4pt}}}
\newcommand{\taninv}{\tan^{-1}}

\begin{document}
	\maketitle
	
	\divline
	
	\begin{multicols}{2}
		\section{Fourier}
		
		\textbf{Main formula}
		
		\[f(t) = a_{0} + \sum_{n = 1}^{\infty} a_{n} \cos{( \frac{2 \pi n}{T} t )} + \sum_{n = 1}^{\infty} b_{n} \sin{( \frac{2 \pi n}{T} t )} \]
		
		\textbf{Orthogonality}
		
		\[ \int_{-\frac{T}{2}}^{\frac{T}{2}} f_{1}(t) f_{2}(t) dt = 
		\begin{cases} 
			\alpha \text{ if } f_{1} = f_{2} \\
			0 \text{ if } f_{1} \neq f_{2}
		\end{cases}
		\]
		
		\textbf{Orthonormality}
		
		\[ \int_{-\frac{T}{2}}^{\frac{T}{2}} (f_{1}(t))^2 dt = 1 \]
		
		The oscillation is named Gibbs phenomenon.
		The equality does not always maintain when operating in both sides.
		
	\end{multicols}
	
	\divline
	
	\begin{multicols}{2}
		\section{Sin and cosine}
		
		Using \(\frac{2}{T}\) to normalize:
		
		\textbf{cos \(\cdot\) cos}
		
		\[ \frac{2}{T} \int_{-\frac{T}{2}}^{\frac{T}{2}} \cos{( \frac{2 n \pi}{T} t )} \cos{( \frac{2 m \pi}{T} t )} dt =
		\begin{cases} 
			0 \text{ if } n \neq 0 \\
			1 \text{ if } n = 0
		\end{cases}
		\]
		
		\textbf{sin \(\cdot\) cos}
		
		\[ \frac{2}{T} \int_{-\frac{T}{2}}^{\frac{T}{2}} \sin{( \frac{2 n \pi}{T} t )} \cos{( \frac{2 m \pi}{T} t )} dt = 0\]
		
		\textbf{sin \(\cdot\) sin}
		
		\[ \frac{2}{T} \int_{-\frac{T}{2}}^{\frac{T}{2}} \sin{( \frac{2 n \pi}{T} t )} \sin{( \frac{2 m \pi}{T} t )} dt =
		\begin{cases} 
			0 \text{ if } n \neq 0 \\
			1 \text{ if } n = 0
		\end{cases}
		\]
		
		\textbf{Applied in Fourier}
		
		\[ \int_{-\frac{T}{2}}^{\frac{T}{2}} f(t) \cos{( \frac{2 n \pi}{T} t )} dt = \sum_{n = 1}^{\infty} a_{n} \cdot \frac{T}{2} \]
		
		\[ \int_{-\frac{T}{2}}^{\frac{T}{2}} f(t) \sin{( \frac{2 n \pi}{T} t )} dt = \sum_{n = 1}^{\infty} b_{n} \cdot \frac{T}{2} \]
		
	\end{multicols}
	
	\divline
	
	\begin{multicols}{2}
		
		\section{Geometric Fourier series}
		
		\[f(t) = a_{0} + \sum_{n = 1}^{\infty} a_{n} \cos{( \frac{2 \pi n}{T} t )} + \sum_{n = 1}^{\infty} b_{n} \sin{( \frac{2 \pi n}{T} t )} \]
		
		Where:
		
		\[a_{0} = \frac{1}{T} \int_{-\frac{T}{2}}^{\frac{T}{2}} f(t) dt \]
		
		\[a_{n} = \frac{2}{T} \int_{-\frac{T}{2}}^{\frac{T}{2}} f(t) \cos{( \frac{2 \pi n}{T} t )} dt \]
		
		\[b_{n} = \frac{2}{T} \int_{-\frac{T}{2}}^{\frac{T}{2}} f(t) \sin{( \frac{2 \pi n}{T} t )} dt \]
		
	\end{multicols}
	
	\divline
	
	\begin{multicols}{3}
		\section{Parity functions}
		
		\textbf{Even:}
		
		\[f(t) = f(-t)\]
		
		For integrals in origin you can calculate half and multiply by 2
		
		\textbf{Odd:}
		
		\[f(t) = - f(-t)\]
		
		Integrals in origin are equal to 0.
		
		\textbf{Properties:}
		
		\[f_{p}(t) \cdot f_{p}(t) = f_{p}(t)\]
		\[f_{i}(t) \cdot f_{i}(t) = f_{p}(t)\]
		\[f_{i}(t) \cdot f_{p}(t) = f_{i}(t)\]
		
		\textbf{In Fourier}
		
		If \(f(t)\) is even:
		
		\[a_{0} = \frac{2}{T} \int_{0}^{\frac{T}{2}} f_{p}(t) dt \]
		\[a_{n} = \frac{4}{T} \int_{0}^{\frac{T}{2}} f_{p}(t) \cos{(\frac{2 n \pi}{T} t)} dt \]
		\[b_{n} = 0\]
		
		If \(f(t)\) is odd:
		
		\[a_{0} = 0\]
		\[a_{n} = 0\]
		\[b_{n} = \frac{4}{T} \int_{0}^{\frac{T}{2}} f_{p}(t) \sin{(\frac{2 n \pi}{T} t)} dt \]
		
	\end{multicols}
	
	\divline
	
	\begin{multicols}{2}
		
		\section{Complex Fourier series}
		
		\[f(t) = \sum_{n = - \infty}^{\infty} C_{n} e^{\frac{i2n\pi}{T} t} \]
		
		Where:
		
		\[C_{n} = \frac{1}{T} \int_{-\frac{T}{2}}^{\frac{T}{2}} f(t) e^{-\frac{i2n\pi}{T}t} dt \]
		
		\[a_{n} = 2 \mathbb{R}\text{e}(C_{n})\]
		\[b_{n} = - 2 \mathbb{I}\text{m}(C_{n})\]
		
	\end{multicols}
	
	\divline
	
\end{document}
