\documentclass[letterpaper]{article}

% --- Packages
\usepackage[utf8]{inputenc}
\usepackage[T1]{fontenc}
\usepackage[margin=0.25cm]{geometry}
\usepackage{enumitem}
\usepackage{pdfpages}
\usepackage{multicol}
\usepackage{amsmath}
\usepackage{amssymb}
\usepackage[skip=1pt plus1pt, indent=0pt]{parskip}
\usepackage{enumitem}
\usepackage{graphicx}

% --- Data
\title{Laplacce}
\author{Enrique Calderon \& Elizabeth Portilla}

% --- Graphics path
\graphicspath{ {./img/} }

% --- Custom commands
\makeatletter
\let\thetitle\@title
\let\theauthor\@author
\makeatother
\newcommand{\compconj}[1]{%
    \overline{#1}%
}
\newcommand{\divline}{\noindent\makebox[\linewidth]{\rule{\textwidth}{0.4pt}}}
\newcommand{\taninv}{\tan^{-1}}

\begin{document}
    \maketitle

    \divline

    \begin{multicols}{2}

        \section{By definition}

            \[\mathcal{L} (f(t)) = F(S) = \int_{0}^{\infty} e^{-St} f(t) dt \]

            or 

            \[F(S) = \lim_{b \to \infty } \int_{0}^{b} e^{-St} f(t) dt \]

            And the inverse

            \[\mathcal{L}^{-1} (F(S)) = f(t) = \frac{1}{2\pi} \int_{-i\infty}^{i\infty} e^{St}F(S) \]
            
    \end{multicols}

    \divline

    \begin{multicols}{2}
        \section{For differential equations}

            \[\mathcal{L} \{ f^{n} (\mathcal{T}) \} = S^{n} F(S) - S^{n-1} f(0) - ... - f^{n-1} (0) \]

            To solve differential equations first convert with Laplace operator, solve it and then apply inverse Laplace operator.

    
    \end{multicols}

    \divline

    \begin{multicols}{2}
        \section{Translation theorem}
            			
		\[u(\mathcal{T}-a) = 
			\begin{cases} 
				0  & 0 \leq t \leq a \\
				1 & 1 \geq a
			\end{cases}
		\]

             \[\mathcal{L} \{ u(\mathcal{T} - a) \} = \frac{e^{-aS}}{S} \]
             
             \[\mathcal{L} \{ f(\mathcal{T} - a) u(\mathcal{T} - a) \} = e^{-aS} F(S) \]

    \end{multicols}

    \divline

    \begin{multicols}{2}
        \section{Dirac's delta}

            \[\delta (\mathcal{T} - \mathcal{T}_{0}) = 
                \begin{cases} 
				0  & 0 \leq \mathcal{T} < \mathcal{T}_{0} - a \\
                    \frac{1}{2}a & \mathcal{T}_{0} - a \leq \mathcal{T} < \mathcal{T}_{0} + a \\
				0 & \mathcal{T}_{0} + a \leq \mathcal{T}
			\end{cases}
            \]

            \[\mathcal{L} \{ \delta(\mathcal{T} - \mathcal{T}_{0}) \} = e^{-\mathcal{T}_{0} S} \]
    \end{multicols}

    \divline

    \begin{multicols}{2}
        \section{Convolution}

            \[f * g = \int^{\mathcal{T}}_0 f(x) g(\mathcal{T} - x) dx \]

            \[\mathcal{L} \{ f * g \} = \mathcal{L} \{ f(\mathcal{T}) \} \mathcal{L} \{ g(\mathcal{T}) \} \]
    \end{multicols}

    \divline

    \begin{multicols}{2}
        \section{Differential equations system}
            1. Solve differential equations separately
            2. Arrange the solutions of each differential equation as a system
            \[ 
                \begin{cases} 
				AX(s) + BY(S) = f_1(S)\\
                CX(s) + DY(S)  = f_2(S)\\
			\end{cases}
            \]
            3. Solve system by Cramer's method to find values of X(s), Y(S)...
            
            \[Y(s) = \frac{
            \begin{vmatrix}
                A & f_1(S)\\
                C & f_2(S)
            \end{vmatrix}}
            {
            \begin{vmatrix}
                A & B\\
                C & D
            \end{vmatrix}
            }\]
            \[X(s) = \frac{
            \begin{vmatrix}
                f_1(S) & B\\
                f_2(S) & D
            \end{vmatrix}}
            {
            \begin{vmatrix}
                A & B\\
                C & D
            \end{vmatrix}
            }\]

            4. Obtaining:
            
             \[{L}^{-1} (X(S)) = X(t)\]  \\
             \[{L}^{-1} (Y(S)) = Y(t) \]
                    
    \end{multicols}
\end{document}
